aver-cert/src/engine/expr_fragment_defs.rs
@@ -394,6 +394,7 @@ pub enum FragPrim {
     I64LeS,
     I64LtS,
     I64GeS,
+    I32Eq,
     I32LtS,
     I32GtS,
 }
@@ -409,6 +410,7 @@ impl FragPrim {
             FragPrim::I64LeS => "i64.le_s",
             FragPrim::I64LtS => "i64.lt_s",
             FragPrim::I64GeS => "i64.ge_s",
+            FragPrim::I32Eq => "i32.eq",
             FragPrim::I32LtS => "i32.lt_s",
             FragPrim::I32GtS => "i32.gt_s",
         }
@@ -424,6 +426,7 @@ impl FragPrim {
             FragPrim::I64LeS => ".i64LeS",
             FragPrim::I64LtS => ".i64LtS",
             FragPrim::I64GeS => ".i64GeS",
+            FragPrim::I32Eq => ".i32Eq",
             FragPrim::I32LtS => ".i32LtS",
             FragPrim::I32GtS => ".i32GtS",
         }
